Phi_Semantics/PhiSem_Variable.thy
@@ -58,7 +58,7 @@ section \<open>\<phi>-Types\<close>
 
 subsection \<open>Variable\<close>
 
-declare [[\<phi>trace_reasoning = 0]]
+declare [[\<phi>trace_reasoning = 1]]
 
 \<phi>type_def Var :: \<open>varname \<Rightarrow> (VAL option,'a) \<phi> \<Rightarrow> (fiction,'a) \<phi>\<close>
   where \<open>Var vname T \<equiv> (FIC.Var.\<phi> (vname \<^bold>\<rightarrow> \<black_circle> (Nosep T)))\<close>
